{
 "cells": [
  {
   "cell_type": "markdown",
   "id": "950985c1",
   "metadata": {},
   "source": [
    "# Assignment 1 - Gradients\n",
    "#### Meir Shamir 326198595"
   ]
  },
  {
   "cell_type": "markdown",
   "id": "dd39d1c6",
   "metadata": {},
   "source": [
    "### 1. Sigmoid Function Gradient\n",
    "\n",
    "#### 1.\n",
    "$$\n",
    "\\sigma(x) = \\frac{1}{1 + e^{-x}}\n",
    "$$\n",
    "$$\n",
    "\\sigma(x) = (1 + e^{-x})^{-1}\n",
    "$$\n",
    "$$\n",
    "\\frac{d\\sigma}{dx} = -1 \\cdot (1 + e^{-x})^{-2} \\cdot \\frac{d}{dx}(1 + e^{-x})\n",
    "$$\n",
    "$$\n",
    "\\frac{d\\sigma}{dx} = -1 \\cdot (1 + e^{-x})^{-2} \\cdot (-e^{-x})\n",
    "$$\n",
    "$$\n",
    "\\frac{d\\sigma}{dx} = \\frac{e^{-x}}{(1 + e^{-x})^2}\n",
    "$$\n",
    "\n",
    "#### 2.\n",
    "$$\n",
    "\\frac{d\\sigma}{dx} = \\left( \\frac{1}{1 + e^{-x}} \\right) \\cdot \\left( \\frac{e^{-x}}{1 + e^{-x}} \\right)\n",
    "$$\n",
    "$$\n",
    "\\frac{1}{1 + e^{-x}} = \\sigma(x)\n",
    "$$\n",
    "$$\n",
    "\\frac{e^{-x}}{1 + e^{-x}} = \\frac{(1 + e^{-x}) - 1}{1 + e^{-x}} = \\frac{1 + e^{-x}}{1 + e^{-x}} - \\frac{1}{1 + e^{-x}} = 1 - \\sigma(x)\n",
    "$$\n",
    "$$\n",
    "\\frac{d\\sigma}{dx} = \\sigma(x)(1 - \\sigma(x))\n",
    "$$"
   ]
  },
  {
   "cell_type": "markdown",
   "id": "b59774c2",
   "metadata": {},
   "source": [
    "### 2. Tanh Function Gradient\n",
    "\n",
    "#### 1.\n",
    "$$\n",
    "\\tanh(x) = \\frac{e^x - e^{-x}}{e^x + e^{-x}} \\quad \\left[ \\text{using } \\frac{f'g - fg'}{g^2} \\right]\n",
    "$$\n",
    "$$\n",
    "f = e^x - e^{-x} \\implies f' = e^x + e^{-x}\n",
    "$$\n",
    "$$\n",
    "g = e^x + e^{-x} \\implies g' = e^x - e^{-x}\n",
    "$$\n",
    "$$\n",
    "\\frac{d\\tanh}{dx} = \\frac{(e^x + e^{-x})(e^x + e^{-x}) - (e^x - e^{-x})(e^x - e^{-x})}{(e^x + e^{-x})^2}\n",
    "$$\n",
    "$$\n",
    "\\frac{d\\tanh}{dx} = \\frac{(e^x + e^{-x})^2 - (e^x - e^{-x})^2}{(e^x + e^{-x})^2}\n",
    "$$\n",
    "\n",
    "#### 2.\n",
    "$$\n",
    "\\frac{d\\tanh}{dx} = \\frac{(e^x + e^{-x})^2}{(e^x + e^{-x})^2} - \\frac{(e^x - e^{-x})^2}{(e^x + e^{-x})^2}\n",
    "$$\n",
    "$$\n",
    "\\frac{d\\tanh}{dx} = 1 - \\left( \\frac{e^x - e^{-x}}{e^x + e^{-x}} \\right)^2\n",
    "$$\n",
    "$$\n",
    "\\frac{d\\tanh}{dx} = 1 - \\tanh(x)^2\n",
    "$$"
   ]
  }
 ],
 "metadata": {
  "language_info": {
   "name": "python"
  }
 },
 "nbformat": 4,
 "nbformat_minor": 5
}
